#-----------------------------------------------------------------------------------------------------------------------
# Copyright 2017  Xerox Research Centre Europe
#
# Licensed under the Apache License, Version 2.0 (the "License");
# you may not use this file except in compliance with the License.
# You may obtain a copy of the License at
#
# 	http://www.apache.org/licenses/LICENSE-2.0
#
# Unless required by applicable law or agreed to in writing, software
# distributed under the License is distributed on an "AS IS" BASIS,
# WITHOUT WARRANTIES OR CONDITIONS OF ANY KIND, either express or implied.
# See the License for the specific language governing permissions and
# limitations under the License.
#-----------------------------------------------------------------------------------------------------------------------

#
# PERICLES (see http://www.pericles-project.eu )is a four-year project that aims to address the challenge of ensuring that digital content remains 
# accessible in an environment that is subject to continual change. This can encompass not only technological change, but also changes in semantics, 
# academic or professional practice, or society itself, which can affect the attitudes and interests of the various stakeholders that interact with the content. 
# PERICLES will take a ‘preservation by design’ approach that involves modelling, capturing and maintaining detailed and complex information about 
# digital content, the environment in which it exists, and the processes and policies to which it is subject.
#
# This ontology has been produced by the WP3 (work package 3)lead by Xerox Research Center Europe 
# Authors:  Jean-Pierre Chanod, Nikolaos Lagos, Jean-Yves Vion-Dury
#
# Created in November 2014
# last updated the 31th of March 2017 by Jean-Yves Vion-Dury
#
@prefix rdf: <http://www.w3.org/1999/02/22-rdf-syntax-ns#> .
@prefix rdfs: <http://www.w3.org/2000/01/rdf-schema#> .
@prefix owl: <http://www.w3.org/2002/07/owl#> .
@prefix xsd: <http://www.w3.org/2001/XMLSchema#> .
@prefix lrm: <http://xrce.xerox.com/LRM#> .

# @base  <file:///C:/Users/viondury/PERICLESEU/Ontology/> .

lrm:LRM-static
    a owl:Ontology;
	owl:versionInfo "2.0.3"    
	.

lrm:Resource a owl:Class;
    owl:disjointUnionOf (lrm:EndogenousResource lrm:ExogenousResource) ;
    rdfs:comment "Endogenous resources talk about the representation system, whereas Exogenous resources talk about the ecosystem"@en;
    owl:disjointUnionOf (lrm:AbstractResource lrm:ConcreteResource) ;
    rdfs:comment """ 
        In our view, abstract resources have no physical extension. However, they may be delimited in time, and thus 
        may have a temporal support; they also may be subject to changes. 
        In our view, concrete resources have a physical and temporal extension.
        As such, they can be located in space and time, and the nature of their physical extension may be described accordingly (e.g. mass, size, volumes, mereological organization...).
        """@en;
    owl:disjointUnionOf (lrm:MutableResource lrm:ImmutableResource) ;
    rdfs:comment "Mutable resources can change"@en,
              "Immutable resources cannot change "@en
    .
    
lrm:AbstractResource rdfs:subClassOf lrm:Resource.
lrm:ConcreteResource rdfs:subClassOf lrm:Resource.

lrm:EndogenousResource rdfs:subClassOf lrm:AbstractResource.
lrm:ExogenousResource rdfs:subClassOf lrm:Resource.
lrm:AbstractExogenousResource rdfs:subClassOf lrm:ExogenousResource, lrm:AbstractResource.

lrm:MutableResource rdfs:subClassOf lrm:Resource.
lrm:ImmutableResource rdfs:subClassOf lrm:Resource.
lrm:DeletedResource rdfs:subClassOf lrm:ImmutableResource.
    
# could be "concretizedAs" and "concretizes"
lrm:realizedAs a owl:ObjectProperty;
    rdfs:domain lrm:AbstractResource;
    rdfs:range lrm:ConcreteResource;
    rdfs:comment "This must be used to link an abstract resource to one or several concrete realizations of it"@en
    .
lrm:realizes owl:inverseOf lrm:realizedAs.


#  -------------------------------------------------------------------------------------------------------------------------------------------------------------------------------------------------------------------------------
#       Description class: Handles Metadata
#  -------------------------------------------------------------------------------------------------------------------------------------------------------------------------------------------------------------------------------
lrm:Description rdfs:subClassOf lrm:EndogenousResource;
    rdfs:comment "gives information about a resource, e.g. why it exists (intention), what it is for (specification),  ... "@en
    .
    
lrm:describedBy rdf:type owl:ObjectProperty;
    rdfs:domain lrm:Resource; 
    rdfs:range lrm:Description
    .
    
lrm:describes owl:inverseOf lrm:describedBy.

lrm:definition a owl:DatatypeProperty;
    rdfs:domain lrm:Resource;
    rdfs:range rdfs:Literal;
    rdfs:comment "This property allows defining formally the resource through a string"@en
    .
    
#  -------------------------------------------------------------------------------------------------------------------------------------------------------------------------------------------------------------------------------
#    Heterogeneous resources: to handle (possibly recursive) aggregated resources - useful to handle mereological models
#  -------------------------------------------------------------------------------------------------------------------------------------------------------------------------------------------------------------------------------
lrm:AggregatedResource rdfs:subClassOf lrm:Resource;
    rdfs:comment "Mereology (from the Greek μερος, 'part') is the theory of parthood relations: of the relations of part to whole and the relations of part to part within a whole."@en;
    rdfs:seeAlso <http://plato.stanford.edu/entries/mereology/>
    .
lrm:hasPart a owl:ObjectProperty, owl:TransitiveProperty;
    rdfs:domain lrm:AggregatedResource;
    rdfs:range lrm:Resource
    .
lrm:partOf owl:inverseOf lrm:hasPart.

#  -------------------------------------------------------------------------------------------------------------------------------------------------------------------------------------------------------------------------------
#  Typology of descriptors
#  -------------------------------------------------------------------------------------------------------------------------------------------------------------------------------------------------------------------------------
lrm:Location rdfs:subClassOf lrm:Description;	
    rdfs:comment """
        Location descriptor is information about retrieving the concrete  resource. 
        """@en .
    
lrm:Protocol rdfs:subClassOf lrm:Description;	
    rdfs:comment """
        explain the method/protocol used to retrieve a concrete  resource (e.g. http, ftp, or an informal textual description). 
        """@en .

lrm:Identity rdfs:subClassOf lrm:Description;
	rdfs:comment """
        The identity of an Resource is uniquely defined via an instance of class lrm:Identity.
        Although the structure of those instances are not defined at this level, it may use 
        UUID mechanisms such as defined in RFC 4122.
        """@en;
    rdfs:seeAlso <http://tools.ietf.org/pdf/rfc4122>
	.
    
# ===================================================================
#       TIME MODEL : fully developped  in time-schema ontology
# ===================================================================
lrm:TemporalDescription rdfs:subClassOf lrm:Description;
    rdfs:comment "Used to provide temporal knowledge about the resource"    
    .
lrm:TimeInterval  rdfs:subClassOf lrm:TemporalDescription.
lrm:TimeInstant  rdfs:subClassOf lrm:TemporalDescription.
lrm:TimeDuration  rdfs:subClassOf lrm:TemporalDescription.

lrm:spanTime a owl:ObjectProperty, owl:FunctionalProperty;
    rdfs:subPropertyOf lrm:describedBy;
    rdfs:domain lrm:Resource;
    rdfs:range lrm:TimeInterval
    .

lrm:creationTime a owl:ObjectProperty, owl:FunctionalProperty;
    rdfs:subPropertyOf lrm:describedBy;
    rdfs:domain lrm:Resource;
    rdfs:range lrm:TimeInstant
    .

lrm:deletionTime a owl:ObjectProperty, owl:FunctionalProperty;
    rdfs:subPropertyOf lrm:describedBy;
    rdfs:domain lrm:Resource;
    rdfs:range lrm:TimeInstant
    .
    
lrm:durationTime a owl:ObjectProperty, owl:FunctionalProperty;
    rdfs:comment "correspond to a duration"@en;
    rdfs:subPropertyOf lrm:describedBy;
    rdfs:domain lrm:Resource;
    rdfs:range lrm:TimeDuration
    .
    
lrm:preceding a owl:ObjectProperty, 
	# added the 09/19/2015 JYVD (once withdrawn because causing troubles to some inference engines)
	# owl:AsymmetricProperty,
	owl:TransitiveProperty;
    rdfs:comment "correspond to a strict causal ordering between any lrm:Resource instances (not time per se, but may be interpreted consistently w.r.t. interval or instant semantic)"@en;
    rdfs:domain lrm:Resource;
    rdfs:range lrm:Resource
    .
    
lrm:following a owl:ObjectProperty, 
	# added the 09/19/2015 JYVD (might be withdrawn because causing troubles to some inference engines)
	# owl:AsymmetricProperty,	
	owl:TransitiveProperty;
    rdfs:comment "correspond to a strict causal ordering between any lrm:Resource instances (not time per se, but may be interpreted consistently w.r.t. interval or instant semantic)"@en;
    owl:inverseOf lrm:preceding;
    rdfs:domain lrm:Resource;
    rdfs:range lrm:Resource
    .
    
lrm:synchronousWith a owl:ObjectProperty, owl:SymmetricProperty, owl:TransitiveProperty;
    rdfs:comment "correspond to a strict time equality between any lrm:Resources instances (interpreted consistently w.r.t. interval or instant semantic)"@en;
    rdfs:domain lrm:Resource;
    rdfs:range lrm:Resource
    .
    
# ===================================================================
#       SPACE MODEL : to be developped and refined if required by applications
# ===================================================================
lrm:SpatialDescription rdfs:subClassOf lrm:Description;
    rdfs:comment "Used to provide spatial knowledge about the resource"    
    .
    
lrm:spaceLocation  a owl:ObjectProperty, owl:FunctionalProperty;
    rdfs:comment "correspond to a place (a point or an area in space )"@en;
    rdfs:subPropertyOf lrm:describedBy;
    rdfs:domain lrm:ConcreteResource;
    rdfs:range lrm:SpatialDescription
    .
    
#  -------------------------------------------------------------------------------------------------------------------------------------------------------------------------------------------------------------------------------
#  linking metadata to resources
#  -------------------------------------------------------------------------------------------------------------------------------------------------------------------------------------------------------------------------------

lrm:identification a owl:ObjectProperty, owl:FunctionalProperty;
    rdfs:subPropertyOf lrm:describedBy;
    rdfs:domain lrm:Resource;
    rdfs:range lrm:Identity;
    rdfs:comment "an Identity instance uniquely identifies a resource (hence the functional property)"@en
    .
    
lrm:location a owl:ObjectProperty;
    rdfs:subPropertyOf lrm:describedBy;
    rdfs:domain lrm:ConcreteResource;
    rdfs:range lrm:Location;
    rdfs:comment "distinct resources cannot have the same location  descriptor(hence the inverse functional property)"@en
    .
        
lrm:accessProtocol a owl:ObjectProperty;
    rdfs:subPropertyOf lrm:describedBy;
    rdfs:domain lrm:Location;
    rdfs:range lrm:Protocol
    .
    
lrm:url a owl:ObjectProperty;
    rdfs:subPropertyOf lrm:describedBy;
    rdfs:comment "The acronym URL stands fo Uniform Resource Locator..."@en;
    rdfs:domain lrm:Location
    .
    
lrm:intention a owl:ObjectProperty, owl:FunctionalProperty;
    rdfs:subPropertyOf lrm:describedBy;
    rdfs:domain lrm:Resource; 
    rdfs:range lrm:Intention ;
    rdfs:comment "This property allows describing, formally or not, the intented usage of the resource (answer to the WHY question)"@en
    .

lrm:Intention 
    rdfs:subClassOf lrm:Description ;
    rdfs:comment """ Used to express the intention usage of the resource (or purpose of...)"""@en  
    .
    
lrm:Specification 
    rdfs:subClassOf lrm:Description ;
    rdfs:comment """
        Used to express the semantical properties. could be a formal logical language, a test-oriented prog. language, a formal or informal policy, a textual description...
        """@en  
    .
    
lrm:specifiedBy
    a owl:ObjectProperty, owl:FunctionalProperty;
    rdfs:subPropertyOf lrm:describedBy;
    owl:inverseOf lrm:specifies ;
    rdfs:domain lrm:Resource;
    rdfs:range lrm:Specification ;
    rdfs:comment """
        This property is used to express, formally or not, the semantical properties of the resource: it must be compatible with the invariant property attached to the resource, if any.
        """@en
    .
    
lrm:invariant 
    a owl:ObjectProperty, owl:FunctionalProperty;
    rdfs:subPropertyOf lrm:describedBy;
    rdfs:comment "specifies what must be always verified along the whole object life."@en;
    rdfs:comment "also relates to the so-called \"significant properties\" used in digital preservation."@en;
    rdfs:seeAlso <http://plato.stanford.edu/entries/identity-time/>;
    rdfs:domain lrm:Resource;
    rdfs:range lrm:Specification
    .
    
    
#  -------------------------------------------------------------------------------------------------------------------------------------------------------------------------------------------------------------------------------
#       DigitalResource class
#  -------------------------------------------------------------------------------------------------------------------------------------------------------------------------------------------------------------------------------
lrm:DigitalResource 
    rdfs:subClassOf lrm:ConcreteResource;
	rdfs:comment """
        A data structure that can be located by a dedicated descriptor, and having
        a unique identifier. The extension of a digital resource is a bit stream that can 
        be fetched using the location descriptor.
        """@en;
    rdfs:seeAlso <http://www.doi.org/handbook_2000/glossary.html>;
	rdfs:comment 
        """Jens[conf. Thibodeau/terminology overview (pericles internal documents)]: 
        a technical object, processable by machines/computers (e.g. a set of files), 
        as opposed to the physical or intellectual object
        """@en;
	rdfs:seeAlso <http://www.clir.org/pubs/reports/pub107/thibodeau.html>;
	rdfs:seeAlso <http://www.doi.org/doi_handbook/Glossary.html>
    .
    
lrm:extension a owl:DatatypeProperty, owl:FunctionalProperty;
    rdfs:subPropertyOf lrm:definition;
    rdfs:domain lrm:DigitalResource;
    rdfs:range rdfs:Literal;
    rdfs:comment "This property allows defining formally the digital extension of a resource (its bit stream)"@en;
    rdfs:seeAlso <http://www.w3.org/TR/Content-in-RDF10>
    .
    
lrm:DigitalSignature rdfs:subClassOf lrm:Description .
    
lrm:fingerprint 
    a owl:ObjectProperty, owl:FunctionalProperty;
    rdfs:subPropertyOf lrm:describedBy;
    rdfs:comment "could be a checksum or any digital signature that uniquely represents the bitstream extension of the digital object"@en;
    rdfs:domain lrm:DigitalResource;
    rdfs:range lrm:DigitalSignature
    .
    
lrm:uniqueIdentification
    a owl:ObjectProperty, owl:FunctionalProperty;    
    rdfs:subPropertyOf lrm:identification;
    rdfs:comment "an Identity instance that uniquely designates the digital object"@en;
    rdfs:domain lrm:DigitalResource;
    rdfs:range  lrm:Identity
    .
    
#  -------------------------------------------------------------------------------------------------------------------------------------------------------------------------------------------------------------------------------
#       Dependency class
#  -------------------------------------------------------------------------------------------------------------------------------------------------------------------------------------------------------------------------------

lrm:Dependency rdfs:subClassOf lrm:EndogenousResource ;
    rdfs:comment """
    A dependency, according to the LRM model, is oriented, and may relate at least one lrm:Resource instance to at 
    least one lrm:Resource instance. One dependency instance may bind several resources together: this captures the
    'co-dependencies' phenomenon, also named 'conjunctive dependencies', meaning that all resources must be considered 
    simultaneously, together as a whole. Disjunctive dependencies are naturally expressed using different instances 
    relating the same set of resources.
    The semantics of the instances of this dependency class is conveyed by an instance of lrm:Plan. This last may give 
    information about the intent (WHY), its specification (WHAT), and how it is satisfied (HOW see lrm:Plan, lrm:Description).
    When 'how' is specified, it involves an Agent to perform the plan.
    """@en
    .
    
lrm:ConjunctiveDependency 
    rdfs:subClassOf lrm:Dependency ;
    rdfs:comment " all 'lrm:from' resources are needed by the 'lrm:to' resources for the intended usage"
    .
    
lrm:DisjunctiveDependency 
    rdfs:subClassOf lrm:Dependency;
    rdfs:comment " only one among the 'lrm:from' resources is needed by the 'lrm:to' resources for the intended usage (can choose anyone)"
    .
    
lrm:Dependency 
    owl:disjointUnionOf ( 
        lrm:ConjunctiveDependency 
        lrm:DisjunctiveDependency 
    ).
    
lrm:from a owl:ObjectProperty;
    rdfs:domain lrm:Dependency; 
    rdfs:range lrm:Resource
    .
    
lrm:to rdf:type owl:ObjectProperty;
    rdfs:domain lrm:Dependency; 
    rdfs:range lrm:Resource
    .

       
lrm:Plan rdfs:subClassOf lrm:Description;
    rdfs:seeAlso <http://www.w3.org/TR/2013/REC-prov-o-20130430/#Plan>;
    rdfs:comment """
        Plans are specialized descriptions intended to be executed by some agent (either human or software based); this is thus a mean to 
        give abstract or concrete operational semantics to dependencies."""@en
    .
    
lrm:implementedBy a owl:ObjectProperty;
    rdfs:comment "useful when a Plan is defined through an exogenous resource, e.g. a source file";
    rdfs:subPropertyOf lrm:realizedAs;
    rdfs:domain lrm:Plan;
    rdfs:range lrm:ConcreteResource
    .
    
lrm:impact 
    rdf:type  owl:ObjectProperty, owl:FunctionalProperty;
    rdfs:domain lrm:Dependency; 
    rdfs:range lrm:Plan ;
    rdfs:comment 
        """Designates the lrm:Plan instance that characterizes how the change of a dependee(s) 
        impacts the depending resource(s): what must be done if the dependency is activated"""@en
    .

lrm:precondition
    rdf:type  owl:ObjectProperty, owl:FunctionalProperty;
    rdfs:domain lrm:Dependency; 
    rdfs:range lrm:Plan ;
    rdfs:comment 
        """Designates the lrm:Plan instance that characterizes the conditions for the change of dependee(s) 
        to trigger a change propagation to depending resources."""@en
    .
    
lrm:Agent rdfs:subClassOf lrm:Resource;
    owl:disjointUnionOf ( lrm:SoftwareAgent lrm:HumanAgent lrm:Organization);
    rdfs:comment "An agent is an entity that performs actions, i.e transformative operations over the exogenous/endogenous ecosystem"@en
    .

lrm:SoftwareAgent rdfs:subClassOf lrm:Agent.

#
#  Basic Classes for Humans ; to be derived further for domain specific needs
#
lrm:HumanAgent rdfs:subClassOf lrm:Agent, lrm:ConcreteResource, lrm:ExogenousResource.
lrm:birthTime a owl:ObjectProperty;
    rdfs:subPropertyOf lrm:creationTime;
    rdfs:domain lrm:HumanAgent;
    rdfs:range lrm:TimeInstant
    .
lrm:deathTime a owl:ObjectProperty;
    rdfs:subPropertyOf lrm:deletionTime;
    rdfs:domain lrm:HumanAgent
    .
lrm:lifeTime a owl:ObjectProperty;
    rdfs:subPropertyOf lrm:durationTime;
    rdfs:domain lrm:HumanAgent
    .

#
#  Basic Classes for Organizations ; to be derived further for domain specific needs
#
lrm:Organization rdfs:subClassOf lrm:AggregatedResource, lrm:Agent.

lrm:hasMember rdfs:subPropertyOf lrm:hasPart;
    rdfs:domain lrm:Organization;
    rdfs:range lrm:Agent
    .

lrm:isMemberOf  rdfs:subPropertyOf lrm:partOf;
    owl:inverseOf lrm:hasMember
    .
    
lrm:Community rdfs:subClassOf lrm:AggregatedResource.
lrm:hasContributor rdfs:subPropertyOf lrm:hasPart;
    rdfs:domain lrm:Community;
    rdfs:range lrm:HumanAgent
    .

lrm:isContributorOf  rdfs:subPropertyOf lrm:partOf;
    owl:inverseOf lrm:hasContributor
    .

