#-----------------------------------------------------------------------------------------------------------------------
# Copyright 2017  Xerox Research Centre Europe
#
# Licensed under the Apache License, Version 2.0 (the "License");
# you may not use this file except in compliance with the License.
# You may obtain a copy of the License at
#
# 	http://www.apache.org/licenses/LICENSE-2.0
#
# Unless required by applicable law or agreed to in writing, software
# distributed under the License is distributed on an "AS IS" BASIS,
# WITHOUT WARRANTIES OR CONDITIONS OF ANY KIND, either express or implied.
# See the License for the specific language governing permissions and
# limitations under the License.
#-----------------------------------------------------------------------------------------------------------------------

#
# PERICLES (see http://www.pericles-project.eu )is a four-year project that aims to address the challenge of ensuring that digital content remains 
# accessible in an environment that is subject to continual change. This can encompass not only technological change, but also changes in semantics, 
# academic or professional practice, or society itself, which can affect the attitudes and interests of the various stakeholders that interact with the content. 
# PERICLES will take a ‘preservation by design’ approach that involves modelling, capturing and maintaining detailed and complex information about 
# digital content, the environment in which it exists, and the processes and policies to which it is subject.
#
# This ontology has been produced by the WP3 (work package 3)lead by Xerox Research Center Europe 
# Authors:  Jean-Pierre Chanod, Nikolaos Lagos, Jean-Yves Vion-Dury
#
# Created in November 2014
# last updated the 31th of March 2017 by Jean-Yves Vion-Dury
#

@prefix rdf: <http://www.w3.org/1999/02/22-rdf-syntax-ns#> .
@prefix rdfs: <http://www.w3.org/2000/01/rdf-schema#> .
@prefix owl: <http://www.w3.org/2002/07/owl#> .
@prefix xsd: <http://www.w3.org/2001/XMLSchema#> .
@prefix lrm: <http://xrce.xerox.com/LRM#> .
@prefix time: <http://xrce.xerox.com/TIME#>.
@prefix real: <http://xrce.xerox.com/ReAL#> .

@base  <https://raw.githubusercontent.com/nikolaosLagos/Linked_Resource_Model/master/> .

lrm:LRM-dynamic	rdf:type owl:Ontology;
	owl:versionInfo "2.0.1";
    rdfs:comment """
    The Dynamic Linked Resource Model (DLRM) aims at describing digital resources for preservation purposes. 
    Dependencies allow to describe the logical interconnexions between resources, and therefore express knowledge regarding the condition and impact
    of a change inside the ecosystem. This knowledge can be directly applied to perform automated updating actions (change propagation according to
    the various semantic of dependency) or can help analyzing the ecosystem model to detect inconsistencies and/or weaknesses to advise the curator 
    on preventive or corrective actions. It also can be used to simulate changes inside the ecosytem and explore the potential consequences (with the help 
    of logical inferences based on the ontological informations).
    """@en
    .


# =================================================================================================
#                                                   CHANGE EVENT MODEL    
# =================================================================================================

lrm:Event rdfs:subClassOf lrm:EndogenousResource, lrm:TimeInstant; 
    owl:disjointUnionOf (lrm:EndogenousEvent lrm:ExogenousEvent);
    rdfs:comment "EndogenousEvent instances talk about Endogenous resources, whereas ExogenousEvent instances talk about Exogenous resources. Note that both are (Abstract) Endogenous resources."@en
    .

lrm:byAgent a owl:ObjectProperty;
    rdfs:domain lrm:Event;
    rdfs:range lrm:Agent;
    rdfs:comment "An event is triggered by an activity, which is performed by an agent (therefore, an event is causally related to an acting entity)"@en
    .

lrm:ActivityLifeEvent 
    rdfs:subClassOf lrm:Event;
    owl:disjointUnionOf (
        lrm:ActivityStarted 
        lrm:ActivityStopped
        lrm:ActivitySuspended
        lrm:ActivityResumed
    )    
    .
lrm:ActivityStarted 
    rdfs:subClassOf lrm:ActivityLifeEvent.
    
lrm:ActivityStopped 
    rdfs:subClassOf lrm:ActivityLifeEvent.
    
lrm:ActivitySuspended 
    rdfs:subClassOf lrm:ActivityLifeEvent.
    
lrm:ActivityResumed 
    rdfs:subClassOf lrm:ActivityLifeEvent.

#
# Communication with endogenous/exogenous activities
#
lrm:Message 
    rdfs:subClassOf lrm:Description;
    rdfs:comment "used to send or receive information from services"
    .
    
lrm:parameter a owl:DatatypeProperty;
	rdfs:comment "used to define the content of a particular message";
    rdfs:subPropertyOf lrm:definition;
    rdfs:domain lrm:Message
    .
#
# Service 
#    
lrm:Service rdfs:subClassOf lrm:Description;
    rdfs:comment "describes a service: name, function, inputs/outputs,.... (yet do be defined)"@en;
    owl:disjointUnionOf ( lrm:ExogenousService lrm:EndogenousService) 
    .
    
lrm:ExogenousService rdfs:subClassOf lrm:Service.
    
lrm:EndogenousService rdfs:subClassOf lrm:Service.

lrm:ServiceInvocation 
    rdfs:subClassOf lrm:EndogenousActivity.

lrm:requestedService a owl:ObjectProperty, owl:FunctionalProperty;
    rdfs:subPropertyOf lrm:describedBy;
    rdfs:domain lrm:ServiceInvocation;
    rdfs:range lrm:Service
    .    
    
lrm:input a owl:ObjectProperty;
    rdfs:subPropertyOf lrm:describedBy;
    rdfs:domain lrm:ServiceInvocation;
    rdfs:range lrm:Message
    .    
lrm:output a owl:ObjectProperty;
    rdfs:subPropertyOf lrm:describedBy;
    owl:propertyDisjointWith lrm:input;
    rdfs:domain lrm:ServiceInvocation;
    rdfs:range lrm:Message
    .    
lrm:result a owl:ObjectProperty;
    rdfs:subPropertyOf lrm:output;
    rdfs:domain lrm:ServiceInvocation;
    rdfs:range lrm:Message
    .        
lrm:error a owl:ObjectProperty;
    rdfs:subPropertyOf lrm:output;
    owl:propertyDisjointWith lrm:result;
    rdfs:domain lrm:ServiceInvocation;
    rdfs:range lrm:Message
    .    
lrm:warning a owl:ObjectProperty;
    rdfs:subPropertyOf lrm:output;
    owl:propertyDisjointWith  lrm:result, lrm:error;
    rdfs:domain lrm:ServiceInvocation;
    rdfs:range lrm:Message
    .    

lrm:timeout a owl:ObjectProperty, owl:FunctionalProperty;
    rdfs:subPropertyOf lrm:describedBy;
    rdfs:domain lrm:ServiceInvocation;
    rdfs:range lrm:TimeDuration
    .    

#
# Periodic event
#    
lrm:RecurringEvent 
    rdfs:subClassOf lrm:Event;
    rdfs:comment "used to model periodic events(max number of occurences may be bounded)"
    .
    
lrm:periodicity a owl:ObjectProperty, owl:FunctionalProperty;
    rdfs:subPropertyOf lrm:describedBy;
    rdfs:domain lrm:RecurringEvent;
    rdfs:range lrm:PeriodicEventDescription
    .
    
lrm:PeriodicEventDescription 
    rdfs:subClassOf lrm:Description.

lrm:period a owl:ObjectProperty, owl:FunctionalProperty;
    rdfs:domain lrm:PeriodicEventDescription;
    rdfs:range lrm:TimeDuration
    .
    
lrm:maxCount a owl:DatatypeProperty, owl:FunctionalProperty;
    rdfs:domain lrm:PeriodicEventDescription;
    rdfs:range xsd:positiveInteger
    .
    
    
lrm:ChangeEvent 
    rdfs:subClassOf lrm:Event, lrm:ChangeDescription;
    rdfs:comment 
        "This specific class of event deals with changes: these particular time instant have a significance with respect to modifications of modeled resources (be they endogenous or exogenous)"@en,
        "used to trigger actions required in order to maintain the internal consistency of LRM instances"@en,
        "also used to remember actions undertaken in order to maintain the internal consistency of LRM instances (provenance)"@en

    .
        
lrm:EndogenousChange 
    rdfs:subClassOf lrm:ChangeEvent, lrm:EndogenousEvent;
    rdfs:comment "Event generated by the underlying system to track and process internal changes"@en
    .
    
lrm:ExogenousChange 
    rdfs:subClassOf lrm:ChangeEvent, lrm:ExogenousEvent;
    # owl:disjointWith lrm:EndogenousChange ;
    rdfs:comment "Event generated through explicit requests to signal changes that occured in the external world"@en
    .
    
lrm:subject a owl:ObjectProperty;
    rdfs:subPropertyOf lrm:describes;
    rdfs:domain lrm:ChangeEvent;
    rdfs:range lrm:Resource;
    rdfs:comment "Defines the resource(s)that changed"@en
    .

lrm:CreationEvent 
    rdfs:subClassOf lrm:ChangeEvent;
    rdfs:comment "A new resource has been created; the lrm:subject designates the class of the created resource"@en;
    rdf:type owl:Restriction;
    owl:onProperty lrm:subject;
    owl:someValuesFrom lrm:EndogenousClass
    .
    
lrm:FreezeEvent 
    rdfs:subClassOf lrm:ChangeEvent;
    rdfs:comment "A resource has been frozen: only meta-descriptors can evolve"@en
    .
    
lrm:UnfreezeEvent 
    rdfs:subClassOf lrm:ChangeEvent;
    owl:disjointWith lrm:FreezeEvent, lrm:CreationEvent;
    rdfs:comment "A resource has been unfrozen: it can evolve again"@en
    .
    
lrm:DestructionEvent 
    rdfs:subClassOf lrm:ChangeEvent;
    owl:disjointWith lrm:FreezeEvent, lrm:CreationEvent, lrm:UnfreezeEvent;
    rdfs:comment "A resource has been deleted"@en
    .
    
lrm:TransformationEvent 
    rdfs:subClassOf lrm:ChangeEvent;
    rdfs:comment 
        "A resource is transformed in the ecosystem, meaning that the resource changed, keeping the same identity"@en,
        "NB: the nature of this transformation can be detailled through subclassing."@en
    .
    
lrm:DerivationEvent
    rdfs:subClassOf lrm:CreationEvent,lrm:TransformationEvent;
    rdfs:comment "A new resource is created, on the basis of other known existing resource(s); e.g. a copy operation, a merge, ... "@en
    .
    
lrm:UpdateEvent 
    rdfs:subClassOf lrm:TransformationEvent;
    rdfs:comment "The resource is updated (e.g. its digital extension changed)"@en
    .

lrm:changeMarker rdf:type lrm:ChangeEvent;
    rdfs:comment "Allows marking a resources as changed"@en
    .   
    
    
lrm:derivedFrom a owl:ObjectProperty;
    rdfs:domain lrm:DerivationEvent;
    rdfs:range lrm:Resource;
    rdfs:comment "used in addition to the lrm:subject property to indicate which other resources are involved in the derivation process"@en
    .

lrm:ChangeDescription 
    rdfs:subClassOf lrm:Description;
    rdfs:comment "Used to describe the differences between two resources"@en
    .
    
lrm:changedBy a owl:ObjectProperty;
    rdfs:subPropertyOf lrm:describedBy;
    rdfs:domain lrm:Resource;
    rdfs:range lrm:ChangeDescription;
    rdfs:comment "used in addition to the lrm:subject property to indicate which other resources are involved in the derivation process"@en
    .

lrm:RDF-Delta
    rdfs:subClassOf lrm:ChangeDescription;
    rdfs:comment "Used to describe the differences between two RDF 'star-shaped' subgraphs (i.e having a common subject) "@en
    .
    
rdf:Statement rdfs:subClassOf lrm:Description.
# lrm:Statement rdfs:subClassOf  rdf:Statement, lrm:Description.
    
rdf:predicate a owl:ObjectProperty;
    rdfs:domain rdf:Statement;
    rdfs:range rdf:Property
    .
    
rdf:object a owl:ObjectProperty;
    rdfs:domain rdf:Statement;
    rdfs:range owl:Thing
    .
    
lrm:deletion a owl:ObjectProperty;
    rdfs:subPropertyOf lrm:describedBy;
    rdfs:domain lrm:RDF-Delta;
    rdfs:range rdf:Statement;
    rdfs:comment "Defines which triples of the resource have been deleted (the rdf:subject predicate is defined by the lrm:subject one) "@en
    .
    
lrm:insertion a owl:ObjectProperty;
    rdfs:subPropertyOf lrm:describedBy;
    rdfs:domain lrm:RDF-Delta;
    rdfs:range rdf:Statement;
    rdfs:comment "Defines which triples of the resource have been inserted (the rdf:subject predicate is defined by the lrm:subject one) "@en
    .

lrm:String-Delta 
    rdfs:subClassOf lrm:ChangeDescription;
    rdfs:comment "Used to describe the differences between two resources"@en
    .
    
lrm:modifiedBy a owl:ObjectProperty;
    rdfs:subPropertyOf lrm:describedBy;
    rdfs:domain lrm:DigitalResource;
    rdfs:range lrm:String-Delta;
    rdfs:comment "used in addition to the lrm:subject property to indicate which other resources are involved in the derivation process"@en
    .
    
lrm:stringInsertion a owl:ObjectProperty;
    rdfs:domain lrm:String-Delta;
    rdfs:range lrm:StringOperation;
    rdfs:comment "should be used only if the target resource has an explicit definition  through the lrm:definition predicate "@en;
    rdfs:seeAlso lrm:definition , <LRM-static-schema.ttl>
    .
	
lrm:stringDeletion a owl:ObjectProperty;
    rdfs:domain lrm:String-Delta;
    rdfs:range lrm:StringOperation;
    rdfs:comment "should be used only if the target resource has an explicit definition through the lrm:definition predicate "@en;
    rdfs:comment "in order to be reversible, the deleted string chunk must be explicit (through the lrm:chunkString property)"@en;
    rdfs:seeAlso lrm:definition , <LRM-static-schema.ttl>
    .
	
lrm:stringMove a owl:ObjectProperty;
    rdfs:domain lrm:String-Delta;
    rdfs:range lrm:StringOperation;
    rdfs:comment "should be used only if the target resource has an explicit definition through the lrm:definition predicate "@en;
    rdfs:seeAlso lrm:definition , <LRM-static-schema.ttl>
    .
    
lrm:stringCopy a owl:ObjectProperty;
    rdfs:domain lrm:String-Delta;
    rdfs:range lrm:StringOperation;
    rdfs:comment "should be used only if the target resource has an explicit definition  through the lrm:definition predicate "@en;
    rdfs:seeAlso lrm:definition , <LRM-static-schema.ttl>
    .

lrm:StringOperation 
    rdfs:subClassOf lrm:Description
    .
    
lrm:originPosition a owl:DatatypeProperty;
    rdfs:comment "the origin offset in the string (0 refers to the start of the string)"@en;
    rdfs:domain lrm:StringOperation;
    rdfs:range xsd:nonNegativeInteger
    .
    
lrm:destinationPosition a owl:DatatypeProperty;
    rdfs:comment "the target offset in the string (0 refers to the start of the string)"@en;
    rdfs:domain lrm:StringOperation;
    rdfs:range xsd:nonNegativeInteger
    .
    
lrm:chunkString a owl:DatatypeProperty;
    rdfs:comment "the substring that have been inserted, deleted, moved or copied"@en;
    rdfs:domain lrm:StringOperation;
    rdfs:range rdfs:Literal
    .
    

lrm:Action 
    rdfs:subClassOf lrm:Plan;
    owl:disjointWith lrm:EventHandler;
    rdfs:comment "allows defining modular constructs"
    .
      
lrm:input-signature a owl:DatatypeProperty, owl:FunctionalProperty;
    rdfs:comment 
        "defines the variables that must be bound when calling the action (order is significant) "@en
        ;
    rdfs:domain lrm:Action;
    rdfs:range real:Signature
    .
    
lrm:output-signature a owl:DatatypeProperty, owl:FunctionalProperty;
    rdfs:comment 
        "defines the variables that will be bound after calling the action (and if the action is successful ; order is significant) "@en
        ;
    rdfs:domain lrm:Action;
    rdfs:range real:Signature
    .
    
lrm:body a owl:ObjectProperty;
    rdfs:subPropertyOf lrm:describedBy;
    rdfs:comment 
        "defines the content of the module (uses the formal parameters defined in the signature)"@en,
        "the chunck will be statically analyzed, and all expansion will be realized when possible"@en,
        "the open variables are translated after unification with signature"@en
        ;
    rdfs:domain lrm:Action;
    rdfs:range real:Template
    .

lrm:HandlingAction 
    rdfs:subClassOf lrm:Action;
    rdfs:comment "allows defining actions which signature are dedicated to event handling (receive the instanciated event IRI as input parameter)";
    owl:intersectionOf (
        [ 
		rdf:type owl:Restriction;
		owl:onProperty lrm:input-signature;
		owl:qualifiedCardinality 1;
		owl:onDataRange real:Signature;
		owl:hasValue "EVENT"^^real:Signature
		]
        [ 
		rdf:type owl:Restriction;
		owl:onProperty lrm:body;
		owl:minQualifiedCardinality 1;
		owl:onClass real:Template;
		]
		)
    .

lrm:EventHandler rdfs:subClassOf lrm:Plan;
    owl:intersectionOf (
        [ 
        rdf:type owl:Restriction;
        owl:onProperty lrm:on;
        owl:minQualifiedCardinality 1;
        owl:onClass lrm:EventsClass
        ]
        [ 
        rdf:type owl:Restriction;
        owl:onProperty lrm:do;
        owl:minQualifiedCardinality 1;
        owl:onClass lrm:HandlingAction
        ]
      )
    .
    
lrm:on a owl:ObjectProperty; 
    rdfs:subPropertyOf lrm:describedBy;
    rdfs:domain lrm:EventHandler;
    # rdfs:range lrm:Event
    rdfs:range lrm:EventsClass
    .
    
lrm:do a owl:ObjectProperty; 
    rdfs:subPropertyOf lrm:describedBy;
    rdfs:domain lrm:EventHandler;
    rdfs:range lrm:HandlingAction
    .
    
# =================================================================================================
#                                                   ACTIVITY MODEL    (with provenance related information)
# =================================================================================================
lrm:Activity rdfs:subClassOf lrm:AbstractResource;
    owl:disjointUnionOf ( lrm:EndogenousActivity  lrm:ExogenousActivity) ;
    rdfs:comment 
        """
An activity is defined as the effect of the actions performed by some agent(s);  as such, it is a blackbox that can be observed and acharacterized through its relationship with the flow of events  that influenced it, and also through the resources it used.
Two particularly distinguished event classes mark the active/inactive status of an activity: begining and termination through lrm:ActivityStarted  and lrm:ActivityStopped, as well as the suspension and resuming via lrm:ActivitySuspended and  lrm:ActivityResumed.
An activity may involve other activities: this can be captured by a specific usage of the lrm:used predicate  that also applies to any kind of resources.
An activity can be described through a Plan description (as in PROV)at various level of detail depending on the domain-specific needs.
The resources created, modified or deleted by an activity can be known on the basis of the corresponding events it generated.
Note also that an activity can be either internal, i.e handled by the endogenous infrastructure to manage dynamicity, or external, i.e. occuring in the ecosystem
                """@en
    .
lrm:EndogenousActivity rdfs:subClassOf lrm:Activity, lrm:EndogenousResource.

# JYVD (14 Dec. 2015) modification proposed in order to make LRMS API more consistent (does not change the logical structure of classes)
lrm:ExogenousActivity rdfs:subClassOf lrm:Activity, lrm:AbstractExogenousResource.
    
lrm:executedBy a owl:ObjectProperty;
    rdfs:domain lrm:Activity;
    rdfs:range lrm:Agent;
    rdfs:comment "Relates the activity to the agent(s) that execute it"@en
    .
    
lrm:executes owl:inverseOf lrm:executedBy.

lrm:triggeredBy a owl:ObjectProperty;
    rdfs:domain lrm:Activity;
    rdfs:range lrm:Event;
    rdfs:comment "Relates the activity to event(s) that triggered it"@en
    .
lrm:triggers a owl:ObjectProperty;
    owl:inverseOf lrm:triggeredBy
    .    

lrm:used a owl:ObjectProperty;
    rdfs:domain lrm:Activity;
    rdfs:range lrm:Resource;
    rdfs:comment "Indicates which resources  have been used by the activity"@en  ;  
    owl:inverseOf lrm:usedBy
    .

lrm:created a owl:ObjectProperty;
    rdfs:domain lrm:Activity;
    rdfs:range lrm:Resource;
    rdfs:comment "Indicates which resources have been created by the activity"@en;        
    owl:inverseOf lrm:createdBy 
    .

lrm:deleted a owl:ObjectProperty;
    rdfs:domain lrm:Activity;
    rdfs:range lrm:Resource;
    rdfs:comment "Indicates which resources have been deleted by the activity"@en ;      
    owl:inverseOf lrm:deletedBy
    .
    
lrm:transformed a owl:ObjectProperty;
    rdfs:domain lrm:Activity;
    rdfs:range lrm:Resource;
    rdfs:comment "Indicates which resources have been modified by the activity"@en ;       
    owl:inverseOf lrm:transformedBy
    .
        
lrm:usedPlan a owl:ObjectProperty, owl:FunctionalProperty;
    rdfs:subPropertyOf lrm:used;
    rdfs:range lrm:Plan;
    rdfs:comment "Indicates which plan is executed by the activity"@en    
    .
    
lrm:emitted a owl:ObjectProperty;
    rdfs:domain lrm:Activity ;
    rdfs:range lrm:Event;
    owl:inverseOf lrm:emittedBy;
    rdfs:comment "Indicates which events were directly produced by the subject activity "@en
    .
    
lrm:received a owl:ObjectProperty;
    rdfs:domain lrm:Activity ;
    rdfs:range lrm:Event;
    owl:inverseOf lrm:receivedBy;
    rdfs:comment "Indicates which events were directly received by the subject activity "@en
    .
    
lrm:activity  a owl:ObjectProperty;
    rdfs:domain lrm:ActivityLifeEvent;
    rdfs:range lrm:Activity;
    rdfs:comment "Indicates which activities is the subject of this activity-life dedicated event "@en
    .
    
lrm:started rdfs:subPropertyOf lrm:activity;
    rdfs:domain lrm:ActivityStarted;
    owl:inverseOf lrm:startedBy;
    rdfs:comment "Indicates which activities were directly triggered by the appearance of the subject event "@en
    .    
    
lrm:resumed rdfs:subPropertyOf lrm:activity;
    rdfs:domain lrm:ActivityResumed;
    owl:inverseOf lrm:resumedBy;
    rdfs:comment "Indicates which activities were directly resumed by the appearance of the subject event "@en
    .    
    
lrm:suspended rdfs:subPropertyOf lrm:activity;
    rdfs:domain lrm:ActivitySuspended;
    owl:inverseOf lrm:suspendedBy;
    rdfs:comment "Indicates which activities were directly suspended by the appearance of the subject event "@en
    .
    
lrm:stopped rdfs:subPropertyOf lrm:activity;
    rdfs:domain lrm:ActivityStopped;
    owl:inverseOf lrm:stoppedBy;
    rdfs:comment "Indicates which activities were directly stopped by the appearance of the subject event "@en
    .
    
lrm:isConsequenceOf a owl:ObjectProperty, owl:TransitiveProperty ;
    rdfs:domain lrm:Event;
    rdfs:range lrm:Event;
    rdfs:comment "Indicates causal relationships between events"@en
    .    


